WIP

cava/Cava/Lib/Retiming.v
@@ -30,24 +30,19 @@ Import ListNotations Circuit.Notations.
 Section WithCava.
   Context `{semantics : Cava}.
   (* make a circuit with repeated delays for each signal *)
-  Fixpoint ndelays {t : type} (n : nat) : Circuit t t :=
+  Fixpoint ndelays (t : type) (n : nat) : Circuit t t :=
     match n with
     | 0 => Id
-    | S m => ndelays m >==> Delay
+    | S m => ndelays t m >==> Delay
     end.
 End WithCava.
 
 (* n is the number of delays on the output, m is the number of delays on the
    loop state *)
 Definition retimed {i o} (n m : nat) (c1 c2 : Circuit i o) : Prop :=
-  (* there exists some way of converting between the loop states of c1 and c2 *)
-  exists (proj21 : value (loops_state c2) -> value (loops_state c1))
-    (proj12 : value (loops_state c1) -> value (loops_state c2)),
-    (forall x, proj12 (proj21 x) = x)
-    (* ...and loopless c1 is equivalent to loopless c2 composed with the delay
-       circuits and the state projections *)
-    /\ cequiv (loopless c1)
-             (Second (Comb proj12)
-                     >==> loopless c2
-                     >==> Par (ndelays n) (ndelays m)
-                     >==> Second (Comb proj21)).
+  exists rvals,
+    cequiv c1
+           (LoopInit (loops_reset_state c2)
+                     ((loopless c2)
+                        >==> chreset (Par (ndelays o n)
+                                          (ndelays (loops_state c2) m)) rvals)).
