cava/Cava/Lib/RetimingProperties.v
@@ -47,64 +47,58 @@ All should be based on phase_retimed!
 
  *)
 
-Lemma split_delay {t1 t2} (r1 : value t1) (r2 : value t2) :
+Lemma split_delay_init {t1 t2} (r1 : value t1) (r2 : value t2) :
   cequiv (DelayInit (t:=t1*t2) (r1, r2)) (Par (DelayInit r1) (DelayInit r2)).
 Proof.
-  exists eq. ssplit; [ solve_is_total | reflexivity | ].
+  exists eq. ssplit; [ reflexivity | ].
   cbn [value circuit_state Par].
   intros; subst; destruct_products. ssplit; reflexivity.
 Qed.
+Lemma split_delay {t1 t2} : cequiv (Delay (t:=t1*t2)) (Par Delay Delay).
+Proof. apply split_delay_init. Qed.
 
-(* This admit is not provable! *)
-Lemma Comb_invertible {i o} (f : value i -> cava (value o)) x :
-  exists y, f y = x.
+Lemma LoopInitCE_Compose_l {i o s t}
+      (c : Circuit t i) (body : Circuit (i * s) (o * s)) r :
+  cequiv (First c >==> LoopInitCE r body)
+         (LoopInitCE r (First c >==> body)).
 Admitted.
 
-Lemma move_delay {i o} (c : Circuit i o) r :
-  is_loop_free c = true ->
+Lemma LoopInit_Compose_l {i o s t}
+      (c : Circuit t i) (body : Circuit (i * s) (o * s)) r :
+  cequiv (c >==> LoopInit r body) (LoopInit r (First c >==> body)).
+Admitted.
+
+Lemma move_delay_init {i o} (c : Circuit i o) r :
   cequiv (DelayInit r >==> c)
          (chreset c (fst (step c (reset_state c) r))
                   >==> DelayInit (snd (step c (reset_state c) r))).
 Proof.
-  revert r; induction c; intros.
-  { (* Comb case *)
-    eexists.
-    Unshelve. 2:cbn.
-    exists (fun s1 s2 => snd s2 = c (fst s1)).
-    cbn [value circuit_state reset_state chreset step fst snd]. simpl_ident.
-    ssplit.
-    { split; [ solve_is_total | ].
-      intros; destruct_products; cbn[fst snd] in *; logical_simplify.
-      lazymatch goal with |- context [?x = c _] => pose proof (Comb_invertible c x) end.
-      logical_simplify; subst; eexists_destruct; cbn [fst snd]; eauto. }
-    { reflexivity. }
-    { intros; logical_simplify. destruct_products; cbn [fst snd] in *; subst.
-      ssplit; reflexivity. } }
-  { (* Compose case *)
-    cbn [is_loop_free] in *.
-    lazymatch goal with H : (_ && _)%bool = true |- _ => apply Bool.andb_true_iff in H end.
-    logical_simplify. autorewrite with circuitsimpl.
-    rewrite IHc1 by auto. rewrite <-(Compose_assoc _ _ c2).
-    rewrite IHc2 by auto. autorewrite with circuitsimpl.
-    cbn [step reset_state fst snd]. reflexivity. }
-  { (* First case *)
-    cbn [is_loop_free value] in *. destruct_products.
-    cbn [reset_state fst snd step]. rewrite !split_delay.
-    cbv [Par]. rewrite First_Second_comm.
-    rewrite <-(Compose_assoc _ _ (First c)), <-First_Compose.
-    rewrite IHc by auto.
-    autorewrite with circuitsimpl; reflexivity. }
-  { (* Second case *)
-    cbn [is_loop_free value] in *. destruct_products.
-    cbn [reset_state fst snd step]. rewrite !split_delay.
-    cbv [Par]. autorewrite with circuitsimpl.
-    rewrite <-(Compose_assoc _ _ (Second c)). rewrite <-Second_Compose.
-    rewrite IHc by auto. cbn [chreset].
-    autorewrite with circuitsimpl; reflexivity. }
-  { (* LoopInitCE case *)
-    cbn [is_loop_free] in *. discriminate. }
-  { (* DelayInit case *)
-    reflexivity. }
+  exists (fun (s1 : value i * value (circuit_state c))
+       (s2 : value (circuit_state (chreset c _)) * value o) =>
+       step c (snd s1) (fst s1) = (from_chreset_state (fst s2), snd s2)).
+  cbn [fst snd reset_state from_chreset_state reset_state chreset
+           circuit_state value].
+  rewrite chreset_reset, from_to_chreset_state.
+  rewrite <-surjective_pairing.
+  ssplit; [ reflexivity | ].
+  intros; destruct_products. cbn [step fst snd] in *.
+  lazymatch goal with H : step _ _ _ = _ |- _ => rewrite H end.
+  ssplit; [ reflexivity | ]. cbn [fst snd].
+  rewrite step_chreset; cbn [fst snd].
+  rewrite from_to_chreset_state.
+  rewrite <-surjective_pairing.
+  reflexivity.
+Qed.
+
+Lemma split_ndelays {t1 t2} n :
+  cequiv (ndelays (t1*t2) n) (Par (ndelays t1 n) (ndelays t2 n)).
+Proof.
+  induction n; cbn [ndelays]; autorewrite with circuitsimpl; [ reflexivity | ].
+  rewrite split_delay, IHn. cbv [Par]. autorewrite with circuitsimpl.
+  eapply Proper_Compose; [ | reflexivity ].
+  rewrite <-(Compose_assoc (First _) (Second _) (First _)).
+  rewrite <-!First_Second_comm. autorewrite with circuitsimpl.
+  reflexivity.
 Qed.
 
 (*
@@ -174,28 +168,27 @@ Lemma Par_Id_r {i o t} (f : Circuit i o) : cequiv (Par (Id (t:=t)) f) (Second f)
 Proof. cbv [Par]. autorewrite with circuitsimpl. reflexivity. Qed.
 Hint Rewrite @Par_Id_r using solve [eauto] : circuitsimpl.
 
-Print Cava.
 Lemma Second_Comb {i o t} f :
   cequiv (Second (Comb f)) (Comb (i:=t*i) (o:=t*o) (fun x => (fst x, f (snd x)))).
 Proof.
-  cbv [cequiv]. cbn. ssplit; intros; [ solve_is_total | reflexivity | ].
-  exists (fun i _ _ => i = 0); ssplit; intros; cbn [step fst snd]; try tauto; lia.
+  exists (fun _ _ => True). cbn [value circuit_state]. ssplit; [ tauto | ].
+  intros; logical_simplify. cbn [step fst snd]. ssplit; tauto.
 Qed.
 Hint Rewrite @Second_Comb using solve [eauto] : pull_comb.
 
 Lemma First_Comb {i o t} f :
   cequiv (First (Comb f)) (Comb (i:=i*t) (o:=o*t) (fun x => (f (fst x), snd x))).
 Proof.
-  cbv [cequiv]. cbn. ssplit; intros; [ reflexivity | ].
-  exists (fun i _ _ => i = 0); ssplit; intros; cbn [step fst snd]; try tauto; lia.
+  exists (fun _ _ => True). cbn [value circuit_state]. ssplit; [ tauto | ].
+  intros; logical_simplify. cbn [step fst snd]. ssplit; tauto.
 Qed.
 Hint Rewrite @First_Comb using solve [eauto] : pull_comb.
 
 Lemma Compose_Comb {i t o} f g :
   cequiv (@Compose _ _ i t o (Comb f) (Comb g)) (Comb (f >=> g)).
 Proof.
-  cbv [cequiv]. cbn. ssplit; intros; [ reflexivity | ].
-  exists (fun i _ _ => i = 0); ssplit; intros; cbn [step fst snd]; try tauto; lia.
+  exists (fun _ _ => True). cbn [value circuit_state]. ssplit; [ tauto | ].
+  intros; logical_simplify. cbn [step fst snd]. ssplit; tauto.
 Qed.
 Hint Rewrite @Compose_Comb using solve [eauto] : pull_comb.
 
@@ -207,30 +200,233 @@ Proof.
 Qed.
 Hint Rewrite @Compose_Comb_r using solve [eauto] : pull_comb.
 
-
-Lemma delays_Comb_comm {i o} (f : value i -> cava (value o)) :
-  wequiv (delays >==> Comb f) (Comb f >==> delays).
+Lemma loopless_loop_free {i o} (c : Circuit i o) :
+  is_loop_free c = true -> cequiv (loopless c) (First c).
 Proof.
-  Print wequiv.
-  Search cequivn.
-  induction i.
-  induction n; cbn [ndelays]; autorewrite with circuitsimplw; [ reflexivity | ].
-  rewrite <-(Compose_assoc_w _ _ _ _ (ndelays _) delays).
+  induction c; cbn [loopless is_loop_free];
+    rewrite ?Bool.andb_true_iff; intros; logical_simplify.
+  { (* Comb *)
+    reflexivity. }
+  { (* Compose *)
+    rewrite IHc1, IHc2 by auto.
+    exists (fun (s1 : unit * value (circuit_state c1) * unit * value (circuit_state c2) * unit)
+         (s2 : value (circuit_state c1) * value (circuit_state c2)) =>
+         s1 = (tt, fst s2, tt, snd s2, tt)).
+    cbn [value circuit_state reset_state loops_state fst snd].
+    ssplit; [ reflexivity | ].
+    intros; subst; destruct_products; cbn [fst snd step].
+    ssplit; reflexivity. }
+  { (* First *)
+    rewrite IHc by auto.
+    exists (fun (s1 : unit * value (circuit_state c) * unit) (s2: value (circuit_state c)) =>
+         s1 = (tt, s2, tt)).
+    cbn [value circuit_state reset_state loops_state fst snd].
+    ssplit; [ reflexivity | ].
+    intros; subst; destruct_products; cbn [fst snd step].
+    ssplit; reflexivity. }
+  { (* Second *)
+    rewrite IHc by auto.
+    exists (fun (s1 : unit * value (circuit_state c) * unit) (s2: value (circuit_state c)) =>
+         s1 = (tt, s2, tt)).
+    cbn [value circuit_state reset_state loops_state fst snd].
+    ssplit; [ reflexivity | ].
+    intros; subst; destruct_products; cbn [fst snd step].
+    ssplit; reflexivity. }
+  { (* Loop *)
+    discriminate. }
+  { (* Delay *)
+    reflexivity. }
 Qed.
 
-Lemma ndelays_Comb_comm {i o} (f : value i -> cava (value o)) n :
-  wequiv (ndelays n >==> Comb f) (Comb f >==> ndelays n).
+About to_chreset_state.
+
+Axiom reassemble_state :
+  forall {i o} (c : Circuit i o), value (circuit_state (loopless c)) -> value (loops_state c) -> value (circuit_state c).
+
+Axiom loops_state_from_circuit_state :
+  forall {i o} (c : Circuit i o), value (circuit_state c) -> value (loops_state c).
+Axiom loopless_state_from_circuit_state :
+  forall {i o} (c : Circuit i o), value (circuit_state c) -> value (circuit_state (loopless c)).
+
+Axiom to_chreset_loops_state :
+  forall {i o} {c : Circuit i o} {r : value (circuit_state c)}, value (loops_state c) -> value (loops_state (chreset c r)).
+Axiom from_chreset_loops_state :
+  forall {i o} {c : Circuit i o} {r : value (circuit_state c)}, value (loops_state (chreset c r)) -> value (loops_state c).
+
+Eval simpl in (fun r c => loops_state (DelayInit r >==> c)).
+Locate swap.
+Eval simpl in
+    (fun i o r c =>
+       Circuit (i * loops_state (DelayInit r >==> c)) (o * loops_state (DelayInit r >==> c))).
+Eval simpl in (fun i o r c =>
+ Circuit (i * loops_state (chreset c (fst (step c (reset_state c) r)) >==> DelayInit (snd (step c (reset_state c) r))))
+         (o * loops_state (chreset c (fst (step c (reset_state c) r)) >==> DelayInit (snd (step c (reset_state c) r))))).
+
+Lemma move_delay_loopless {i o} (c : Circuit i o) r :
+  cequiv (loopless (DelayInit r >==> c))
+         (Second (Comb (i:=(tzero*loops_state c))
+                       (o:=(loops_state (chreset c _)*tzero))
+                       (fun x => (to_chreset_loops_state (snd x), tt)))
+            >==> (loopless
+                    (chreset c (fst (step c (reset_state c) r))
+                             >==> DelayInit (snd (step c (reset_state c) r))))
+            >==> Second (Comb (i:=(loops_state (chreset c _)*tzero))
+                              (o:=(tzero * loops_state c))
+                              (fun x => (tt, from_chreset_loops_state (fst x))))).
+Admitted.
+(*
+(* i, (s1, s2)
+
+   == First c1 >==> Second (Comb (fun s => snd s)) >==> loopless c2
+*)
+Lemma loopless_Compose_loop_free_l {i o t} (c1 : Circuit i t) (c2 : Circuit t o) :
+  is_loop_free c1 = true ->
+  cequiv (loopless (c1 >==> c2))
+         ((First c1)
+            >==> (Comb (i:=t*(loops_state c1*loops_state c2)) (o:=_*_*_) (fun '(t,s1,s2) => (t,s2,s1)
+            (fun 
+         ) >==> loopless c2).
+ (Second c1 >==> loopless c2).
+  
+  loopless (Delay >==> c2)
+*)
+Lemma loopless_chreset {i o} (c : Circuit i o) r :
+  cequiv (loopless (chreset c r))
+         (Second (Comb from_chreset_loops_state)
+                 >==> chreset (loopless c) (loopless_state_from_circuit_state c r)
+                 >==> Second (Comb to_chreset_loops_state)).
+Admitted.
+
+Lemma ndelays_succ_l {t} n : cequiv (ndelays t (S n)) (Delay >==> ndelays t n).
 Proof.
-  induction n; cbn [ndelays]; autorewrite with circuitsimplw; [ reflexivity | ].
-  rewrite <-(Compose_assoc_w _ _ _ _ (ndelays _) delays).
+  induction n; cbn [ndelays]; autorewrite with circuitsimpl; [ reflexivity | ].
+  rewrite <-IHn. reflexivity.
 Qed.
 
-Lemma Comb_ext {i o} (f g : value i -> cava (value o)) :
-  (forall x, f x = g x) -> wequiv (Comb f) (Comb g).
+Fixpoint Forall_ndelays {t1 t2 n} (R : value t1 -> value t2 -> Prop)
+  : value (circuit_state (ndelays t1 n))
+    -> value (circuit_state (ndelays t2 n)) -> Prop :=
+  match n with
+  | 0 => fun _ _ => True
+  | S _ =>
+    fun d1 d2 =>
+      Forall_ndelays R (fst d1) (fst d2) /\ R (snd d1) (snd d2)
+  end.
+
+Lemma reassemble_reset_state {i o} (c : Circuit i o) :
+  reassemble_state c (reset_state (loopless c)) (loops_reset_state c) = reset_state c.
+Admitted.
+
+(* TODO: this should be cequiv ==> cequiv ==> iff *)
+Instance Proper_retimed {i o} n m :
+  Proper (cequiv ==> eq ==> iff) (@retimed i o n m).
 Proof.
-  intro Hext. cbv [wequiv]. cbn. ssplit; intros; [ reflexivity | ].
-  exists (fun i _ _ => i = 0); ssplit; intros; cbn [step fst snd]; auto; lia.
+  intros a b Hab c d Hcd. subst. cbv [retimed].
+  split.
+  { intros [r Hac]; logical_simplify.
+    exists r. rewrite <-Hab, Hac. reflexivity. }
+  { intros [r Hbd]; logical_simplify.
+    exists r. rewrite Hab, Hbd. reflexivity. }
 Qed.
+
+Lemma retimed_trans {i o} n m n' m' (c1 c2 c3 : Circuit i o) :
+  retimed n m c1 c2 -> retimed n' m' c2 c3 ->
+  retimed (n + n') (m + m') c1 c3.
+Admitted.
+
+Lemma delay1_output {i o} n m (c1 c2 : Circuit i o) :
+  retimed n m c1 (c2 >==> Delay) ->
+  retimed (S n) m c1 c2.
+Proof.
+  intros.
+  replace (S n) with (n + 1) by lia. replace m with (m + 0) by lia.
+  eapply retimed_trans; [ eassumption | ].
+  cbv [retimed]. cbn [Par circuit_state chreset value ndelays Id].
+  exists (tt, defaultValue, tt). cbn [fst snd].
+  autorewrite with circuitsimpl.
+  change defaultValue with (reset_state (Delay (t:=o))).
+  rewrite chreset_noop, LoopInit_First_r.
+  rewrite <-extract_loops. reflexivity.
+Qed.
+
+Lemma delay1_input {i o} n m (c1 c2 : Circuit i o) :
+  retimed n m c1 (Delay >==> c2) ->
+  retimed (S n) m c1 (chreset c2 (fst (step c2 (reset_state c2) defaultValue))).
+Proof.
+  intros.
+  replace (S n) with (n + 1) by lia.
+  replace m with (m + 0) by lia.
+  eapply retimed_trans; [ eassumption | ].
+  cbv [Delay]. rewrite move_delay_init.
+  cbv [retimed]. cbn [Par circuit_state chreset value ndelays Id Delay].
+  exists (tt, snd (step c2 (reset_state c2) defaultValue), tt). cbn [fst snd].
+  autorewrite with circuitsimpl.
+  rewrite LoopInit_First_r. rewrite <-extract_loops.
+  reflexivity.
+Qed.
+
+Require Import Coq.derive.Derive.
+
+Local Ltac simpl_resets :=
+  cbn [step fst snd defaultValue default_value
+            CombinationalSemantics defaultSignal defaultCombValue].
+
+Derive pipelined_nand
+       SuchThat (retimed
+                   2 0 pipelined_nand
+                   (Comb (i:=Bit*Bit) (o:=Bit) and2
+                         >==> Comb (o:=Bit) inv))
+       As pipelined_nand_correct.
+Proof.
+  (* insert a delay *)
+  apply delay1_input.
+  (* move the delay to the end of the circuit *)
+  rewrite move_delays by reflexivity.
+  (* insert another delay *)
+  apply delay1_input.
+  (* move the delay in between the and2 and inv *)
+  rewrite !Compose_assoc_w.
+  rewrite move_delays by reflexivity.
+  (* reflexivity *)
+  subst pipelined_nand. reflexivity.
+Qed.
+Print pipelined_nand.
+Check pipelined_nand_correct.
+
+Definition cipher_middle_round
+           {state key : type}
+           (sbytes : Circuit state state)
+           (shrows : Circuit state state)
+           (mxcols : Circuit state state)
+           (add_rk : Circuit (state * key) state)
+  : Circuit (state * key) state :=
+  First (sbytes >==> shrows >==> mxcols) >==> add_rk.
+
+Derive retimed_cipher_middle_round
+       SuchThat
+       (forall {state key} n
+          (sbytes retimed_sbytes shrows mxcols : Circuit state state)
+          (add_rk : Circuit (state * key) state),
+           phase_retimed 0 n retimed_sbytes sbytes ->
+           phase_retimed
+             0 n
+             (retimed_cipher_middle_round
+                state key retimed_sbytes shrows mxcols add_rk)
+             (cipher_middle_round sbytes shrows mxcols add_rk))
+       As retimed_cipher_middle_round_correct.
+Proof.
+  intros. cbv [cipher_middle_round].
+  autorewrite with circuitsimplw.
+  eapply delayn_input.
+  cbv [phase_retimed] in * |- . logical_simplify.
+  destruct_lists_by_length. cbn [ndelays] in *.
+  cbv [Par] in *; autorewrite with circuitsimplw in *.
+  rewrite ndelays_First.
+  Print phase_retimed.
+
+  (* TODO: not quite working right now, how to properly incorporate retimed
+     subcomponents? *)
+Abort.
 
 Lemma loopless_LoopInit {i o s} (body : Circuit (i * s) (o * s)) r :
   wequiv (loopless (LoopInit r body))
@@ -295,12 +491,6 @@ Proof.
     with (Id (t:=loops_state c)).
   autorewrite with circuitsimplw. reflexivity.
 Qed.
-
-Axiom reassemble_state :
-  forall {i o} (c : Circuit i o), value (circuit_state (loopless c)) -> value (loops_state c) -> value (circuit_state c).
-
-Axiom loops_state_from_circuit_state :
-  forall {i o} (c : Circuit i o), value (circuit_state c) -> value (loops_state c).
 
 Global Instance Proper_phase_retimed {i o} :
   Proper (eq ==> eq ==> wequiv ==> wequiv ==> iff) (@phase_retimed i o).
