cava/Cava/Lib/CircuitTransformsProperties.v
@@ -37,13 +37,13 @@ Local Ltac simplify :=
 
 Lemma First_Id {t1 t2} : @cequiv (t1 * t2) (t1 * t2) (First Id) Id.
 Proof.
-  exists eq. ssplit; [ solve_is_total | reflexivity | ]. simplify. ssplit; reflexivity.
+  exists eq. ssplit; [ reflexivity | ]. simplify. ssplit; reflexivity.
 Qed.
 Hint Rewrite @First_Id using solve [eauto] : circuitsimpl.
 
 Lemma Second_Id {t1 t2} : @cequiv (t1 * t2) (t1 * t2) (Second Id) Id.
 Proof.
-  exists eq. ssplit; [ solve_is_total | reflexivity | ]. simplify. ssplit; reflexivity.
+  exists eq. ssplit; [ reflexivity | ]. simplify. ssplit; reflexivity.
 Qed.
 Hint Rewrite @Second_Id using solve [eauto] : circuitsimpl.
 
@@ -52,7 +52,7 @@ Proof.
   exists (fun (st1 : unit * value (circuit_state c))
        (st2 : value (circuit_state c)) => st1 = (tt, st2)).
   cbn [value circuit_state Id] in *.
-  ssplit; [ solve_is_total | reflexivity | ]. simplify. ssplit; reflexivity.
+  ssplit; [ reflexivity | ]. simplify. ssplit; reflexivity.
 Qed.
 Hint Rewrite @Compose_Id_l using solve [eauto] : circuitsimpl.
 
@@ -61,7 +61,7 @@ Proof.
   exists (fun (st1 : value (circuit_state c) * unit)
        (st2 : value (circuit_state c)) => st1 = (st2, tt)).
   cbn [value circuit_state Id] in *.
-  ssplit; [ solve_is_total | reflexivity | ]. simplify. ssplit; reflexivity.
+  ssplit; [ reflexivity | ]. simplify. ssplit; reflexivity.
 Qed.
 Hint Rewrite @Compose_Id_r using solve [eauto] : circuitsimpl.
 
@@ -73,37 +73,37 @@ Proof.
        (st2 : value (circuit_state f) * value (circuit_state g) * value (circuit_state h)) =>
        st1 = (fst (fst st2), (snd (fst st2), snd st2))).
   cbn [value circuit_state Id] in *.
-  ssplit; [ solve_is_total | reflexivity | ]. simplify. ssplit; reflexivity.
+  ssplit; [ reflexivity | ]. simplify. ssplit; reflexivity.
 Qed.
 Hint Rewrite @Compose_assoc : circuitsimpl.
 
 Lemma First_Compose {A B C D} (f : Circuit A B) (g : Circuit B C) :
   @cequiv (A * D) (C * D) (First (f >==> g)) (First f >==> First g).
 Proof.
-  exists eq. ssplit; [ solve_is_total | reflexivity | ]. simplify. ssplit; reflexivity.
+  exists eq. ssplit; [ reflexivity | ]. simplify. ssplit; reflexivity.
 Qed.
 Hint Rewrite @First_Compose using solve [eauto] : circuitsimpl.
 
 Lemma Second_Compose {A B C D} (f : Circuit A B) (g : Circuit B C) :
   @cequiv (D * A) (D * C) (Second (f >==> g)) (Second f >==> Second g).
 Proof.
-  exists eq. ssplit; [ solve_is_total | reflexivity | ]. simplify. ssplit; reflexivity.
+  exists eq. ssplit; [ reflexivity | ]. simplify. ssplit; reflexivity.
 Qed.
 Hint Rewrite @Second_Compose using solve [eauto] : circuitsimpl.
 
-Lemma LoopInitCE_First_r {A B C} (s : SignalType) reset
+Lemma LoopInitCE_First_r {A B C} (s : type) reset
       (body : Circuit (A * s) (B * s)) (f : Circuit B C) :
   cequiv (LoopInitCE reset (body >==> First f)) (LoopInitCE reset body >==> f).
 Proof.
-  exists (fun (st1 : value (circuit_state body) * value (circuit_state f) * combType s)
-       (st2 : value (circuit_state body) * combType s * value (circuit_state f)) =>
+  exists (fun (st1 : value (circuit_state body) * value (circuit_state f) * value s)
+       (st2 : value (circuit_state body) * value s * value (circuit_state f)) =>
        st1 = (fst (fst st2), snd st2, snd (fst st2))).
   cbn [value circuit_state] in *.
-  ssplit; [ solve_is_total | reflexivity | ]. simplify. ssplit; reflexivity.
+  ssplit; [ reflexivity | ]. simplify. ssplit; reflexivity.
 Qed.
 Hint Rewrite @LoopInitCE_First_r using solve [eauto] : push_loop.
 
-Lemma LoopInit_First_r {A B C} (s : SignalType) reset
+Lemma LoopInit_First_r {A B C} (s : type) reset
       (body : Circuit (A * s) (B * s)) (f : Circuit B C) :
   cequiv (LoopInit reset (body >==> First f)) (LoopInit reset body >==> f).
 Proof.
@@ -111,13 +111,13 @@ Proof.
 Qed.
 Hint Rewrite @LoopInit_First_r using solve [eauto] : push_loop.
 
-Lemma LoopCE_First_r {A B C} (s : SignalType)
+Lemma LoopCE_First_r {A B C} (s : type)
       (body : Circuit (A * s) (B * s)) (f : Circuit B C) :
   cequiv (LoopCE (body >==> First f)) (LoopCE body >==> f).
 Proof. apply LoopInitCE_First_r. Qed.
 Hint Rewrite @LoopCE_First_r using solve [eauto] : push_loop.
 
-Lemma Loop_First_r {A B C} (s : SignalType)
+Lemma Loop_First_r {A B C} (s : type)
       (body : Circuit (A * s) (B * s)) (f : Circuit B C) :
   cequiv (Loop (body >==> First f)) (Loop body >==> f).
 Proof. apply LoopInit_First_r. Qed.
@@ -161,7 +161,7 @@ Hint Rewrite @Par_Id_r using solve [eauto] : circuitsimpl.
 Lemma Second_Comb {i o t} f :
   cequiv (Second (Comb f)) (Comb (i:=t*i) (o:=t*o) (fun x => (fst x, f (snd x)))).
 Proof.
-  exists (fun _ _ => True). ssplit; [ solve_is_total | tauto | ].
+  exists (fun _ _ => True). ssplit; [ tauto | ].
   cbn [value circuit_state]; intros. destruct_products. logical_simplify.
   ssplit; reflexivity.
 Qed.
@@ -170,7 +170,7 @@ Hint Rewrite @Second_Comb using solve [eauto] : pull_comb.
 Lemma First_Comb {i o t} f :
   cequiv (First (Comb f)) (Comb (i:=i*t) (o:=o*t) (fun x => (f (fst x), snd x))).
 Proof.
-  exists (fun _ _ => True). ssplit; [ solve_is_total | tauto | ].
+  exists (fun _ _ => True). ssplit; [ tauto | ].
   cbn [value circuit_state]; intros. destruct_products. logical_simplify.
   ssplit; reflexivity.
 Qed.
@@ -180,7 +180,7 @@ Lemma Compose_Comb {i t o} f g :
   cequiv (@Compose _ _ i t o (Comb f) (Comb g)) (Comb (f >=> g)).
 Proof.
   exists (fun _ _ => True). cbn [value circuit_state].
-  ssplit; [ solve_is_total | tauto | ].
+  ssplit; [ tauto | ].
   cbn [value circuit_state]; intros. destruct_products. logical_simplify.
   ssplit; reflexivity.
 Qed.
@@ -200,7 +200,7 @@ Proof.
   exists (fun (s1 : value (circuit_state c1) * value (circuit_state c2)) s2 =>
        s1 = (snd s2, fst s2)).
   cbn [value circuit_state].
-  ssplit; [ solve_is_total | reflexivity | ].
+  ssplit; [ reflexivity | ].
   intros; destruct_products. cbn [fst snd] in *.
   logical_simplify. ssplit; reflexivity.
 Qed.
@@ -209,7 +209,7 @@ Hint Rewrite <- @First_Second_comm using solve [eauto] : circuitsimpl.
 Lemma Comb_ext {i o} (f g : value i -> cava (value o)) :
   (forall x, f x = g x) -> cequiv (Comb f) (Comb g).
 Proof.
-  intro Hfg. exists (fun _ _ => True). ssplit; [ solve_is_total | tauto | ].
+  intro Hfg. exists (fun _ _ => True). ssplit; [ tauto | ].
   cbn [value circuit_state]; intros. destruct_products. logical_simplify.
   cbn [step]. rewrite Hfg.
   ssplit; [ reflexivity | tauto ].
